src/DY.Core.Attacker.Knowledge.fst
@@ -112,7 +112,7 @@ val corrupted_state_is_publishable:
     state_was_set tr prin sess_id content /\
     trace_invariant preds tr
   )
-  (ensures is_publishable preds.pr tr content)
+  (ensures is_publishable preds.crypto_preds tr content)
 let corrupted_state_is_publishable preds tr prin sess_id content =
   state_is_knowable_by preds tr prin sess_id content
 
@@ -125,24 +125,24 @@ val attacker_only_knows_publishable_values_aux:
     trace_invariant preds tr /\
     attacker_knows_aux step tr msg
   )
-  (ensures is_publishable preds.pr tr msg)
+  (ensures is_publishable preds.crypto_preds tr msg)
 let rec attacker_only_knows_publishable_values_aux preds step tr msg =
   if step = 0 then (
     FStar.Classical.forall_intro   (FStar.Classical.move_requires   (msg_sent_on_network_are_publishable preds tr));
     FStar.Classical.forall_intro   (FStar.Classical.move_requires   (msg_sent_on_network_are_publishable preds tr));
     FStar.Classical.forall_intro_3 (FStar.Classical.move_requires_3 (corrupted_state_is_publishable preds tr));
-    FStar.Classical.forall_intro   (FStar.Classical.move_requires   (literal_to_bytes_is_publishable preds.pr tr))
+    FStar.Classical.forall_intro   (FStar.Classical.move_requires   (literal_to_bytes_is_publishable preds.crypto_preds tr))
   ) else (
     FStar.Classical.forall_intro   (FStar.Classical.move_requires   (attacker_only_knows_publishable_values_aux preds (step-1) tr));
-    FStar.Classical.forall_intro_2 (FStar.Classical.move_requires_2 (concat_preserves_publishability preds.pr tr));
-    FStar.Classical.forall_intro_2 (FStar.Classical.move_requires_2 (split_preserves_publishability preds.pr tr));
-    FStar.Classical.forall_intro_4 (                move_requires_4 (aead_enc_preserves_publishability preds.pr tr));
-    FStar.Classical.forall_intro_4 (                move_requires_4 (aead_dec_preserves_publishability preds.pr tr));
-    FStar.Classical.forall_intro   (FStar.Classical.move_requires   (pk_preserves_publishability preds.pr tr));
-    FStar.Classical.forall_intro_3 (FStar.Classical.move_requires_3 (pk_enc_preserves_publishability preds.pr tr));
-    FStar.Classical.forall_intro_2 (FStar.Classical.move_requires_2 (pk_dec_preserves_publishability preds.pr tr));
-    FStar.Classical.forall_intro   (FStar.Classical.move_requires   (vk_preserves_publishability preds.pr tr));
-    FStar.Classical.forall_intro_3 (FStar.Classical.move_requires_3 (sign_preserves_publishability preds.pr tr));
+    FStar.Classical.forall_intro_2 (FStar.Classical.move_requires_2 (concat_preserves_publishability preds.crypto_preds tr));
+    FStar.Classical.forall_intro_2 (FStar.Classical.move_requires_2 (split_preserves_publishability preds.crypto_preds tr));
+    FStar.Classical.forall_intro_4 (                move_requires_4 (aead_enc_preserves_publishability preds.crypto_preds tr));
+    FStar.Classical.forall_intro_4 (                move_requires_4 (aead_dec_preserves_publishability preds.crypto_preds tr));
+    FStar.Classical.forall_intro   (FStar.Classical.move_requires   (pk_preserves_publishability preds.crypto_preds tr));
+    FStar.Classical.forall_intro_3 (FStar.Classical.move_requires_3 (pk_enc_preserves_publishability preds.crypto_preds tr));
+    FStar.Classical.forall_intro_2 (FStar.Classical.move_requires_2 (pk_dec_preserves_publishability preds.crypto_preds tr));
+    FStar.Classical.forall_intro   (FStar.Classical.move_requires   (vk_preserves_publishability preds.crypto_preds tr));
+    FStar.Classical.forall_intro_3 (FStar.Classical.move_requires_3 (sign_preserves_publishability preds.crypto_preds tr));
     ()
   )
 #pop-options
@@ -155,10 +155,10 @@ val attacker_only_knows_publishable_values:
     trace_invariant preds tr /\
     attacker_knows tr msg
   )
-  (ensures is_publishable preds.pr tr msg)
+  (ensures is_publishable preds.crypto_preds tr msg)
 let attacker_only_knows_publishable_values preds tr msg =
   eliminate exists step. attacker_knows_aux step tr msg
-  returns is_publishable preds.pr tr msg
+  returns is_publishable preds.crypto_preds tr msg
   with _. (
     attacker_only_knows_publishable_values_aux preds step tr msg
   )
